partial work in tpl

tpl/type_reconstruct.v
@@ -208,6 +208,7 @@ Definition gen_typ (id: typ_id) : typ * typ_id :=
 (* Now we define the algorithm to generate type constraint from a type *)
 Definition typ_constraint := list (typ * typ).
 
+Import List.ListNotations.
 Open Scope list_scope.
 
 Fixpoint reconstruct
@@ -237,10 +238,14 @@ Fixpoint reconstruct
     let (s'', C'') := reconstruct Γ then_ T s' C' in
     let (s''', C''') := reconstruct Γ else_ T s'' C'' in
     (s''', C''')
-  | TTru => (s, (T ,TyBool) :: C)
+  | TTru => (s, (T, TyBool) :: C)
   | TFls => (s, (T, TyBool) :: C)
   end.
 
+Compute reconstruct empty_ctx {{ if (λ x: T, x) y then y else y }}
+        (TyBase "V") 0 [].
+
+Definition subst_typ_fun := typ -> typ.
 
 Fixpoint subst_typ (from: typ) (to: typ) (t: typ) : typ :=
   match t with
@@ -255,4 +260,76 @@ Fixpoint subst_typ (from: typ) (to: typ) (t: typ) : typ :=
   | TyFun a b => TyFun (subst_typ from to a) (subst_typ from to b)
   end.
 
-Definition subst_typ_fun := typ -> typ.
+Fixpoint subst_typ_in_constraint
+         (from: typ) (to: typ) (C: typ_constraint) : typ_constraint :=
+  match C with
+  | [] => []
+  | (a,b) :: s =>
+    (subst_typ from to a, subst_typ from to b)
+      :: (subst_typ_in_constraint from to s)
+  end.
+
+Fixpoint typ_size (t: typ) : nat :=
+  match t with
+  | TyBool => 1
+  | TyBase _ => 1
+  | TyFun a b => 1 + typ_size a + typ_size b
+  end.
+
+Fixpoint constr_size (C: typ_constraint) : nat :=
+  match C with
+  | [] => 0
+  | (a,b) :: C' => typ_size a + typ_size b + constr_size C'
+  end.
+
+Fixpoint fv (t: typ) := admit.
+
+
+Fixpoint fv_count (C: typ_constraint) : nat := admit.
+
+Require Import Program.
+Require Import Wf.
+
+Program Fixpoint unify (C: typ_constraint) (f: subst_typ_fun)
+        {measure {fv_count C, constr_size C}} :=
+  match C with
+  | [] => Some f
+  | ((a,b) :: xs) =>
+    match a, b with
+    | TyBool, TyBool => Some f
+    | TyBool, TyBase _ =>
+      unify (subst_typ_in_constraint b a xs) (fun t => subst_typ b a (f t))
+    | TyBool, TyFun _ _ => None
+    | TyBase _, TyBool =>
+      unify (subst_typ_in_constraint a b xs) (fun t => subst_typ a b (f t))
+    | TyBase a', TyBase b' =>
+      if String.eqb a' b'
+      then unify xs f
+      else unify (subst_typ_in_constraint a b xs) (fun t => subst_typ a b (f t))
+    | TyBase _, TyFun _ _ =>
+      unify (subst_typ_in_constraint a b xs) (fun t => subst_typ a b (f t))
+    | TyFun a1 a2, TyFun b1 b2 =>
+      unify ((a1,b1) :: (a2, b2) :: xs) (fun t => subst_typ b a (f t))
+    | _, _ => None
+    end
+  end
+.
+Next Obligation.
+  induction xs.
+  - simpl. auto.
+  - simpl. destruct a0. simpl.
+
+  apply unify_decreasing. reflexivity.
+Qed.
+
+Check unify.
+
+Definition empty_typ_constraint : typ_constraint := [].
+Definition empty_subst_typ_fun : subst_typ_fun := fun x => x.
+
+
+Compute let (_, constr) :=
+            reconstruct empty_ctx
+                        {{ if (λ x: T, x) y then y else y }}
+                        (TyBase "V") 0 []
+        in unify constr empty_subst_typ_fun (TyBase "V").
