tpl/halting.v
@@ -1,0 +1,185 @@
+(* untyped lambda calculus *)
+
+Require Import Coq.Strings.String.
+Require Import Coq.Strings.Ascii.
+Open Scope string_scope.
+
+
+Inductive term :=
+| TVar (var: string) : term
+| TLam (var: string) (body: term) : term
+| TApp (rator: term) (rand: term) : term
+.
+
+Declare Custom Entry term.
+
+Notation "{{ x }}" := x (x custom term).
+Notation "( x )" := x (in custom term, x custom term).
+
+Notation "'λ' a , body" :=
+  (TLam a body) (in custom term at level 98
+                      , a constr at level 0  (* avoid ":" being interpreted as type *)
+                      , body custom term at level 99
+                      , right associativity).
+
+Notation "t1 t2" :=
+  (TApp t1 t2) (in custom term at level 97
+                   , t1 custom term
+                   , t2 custom term
+                   , left associativity).
+
+Coercion TVar : string >-> term.
+
+Inductive value : term -> Prop :=
+| VLam : forall x t, value (TLam x t)
+.
+Hint Constructors value.
+
+Fixpoint sub (t: term) (x: string) (v: term) :=
+  match t with
+  | TLam x' t' => if String.eqb x x'
+                 then TLam x' t'
+                 else TLam x' (sub t' x v)
+  | TVar x' => if  String.eqb x x'
+              then v
+              else x'
+  | TApp t1 t2 => TApp (sub t1 x v) (sub t2 x v)
+  end.
+
+Notation "[ x '|->' v ] t" :=
+  (sub t x v) ( in custom term at level 96
+                   , t custom term
+                   , v custom term
+                   , x constr at level 0
+                   , right associativity
+              ).
+
+(* the ~value terms are not necessary, but I don't want to bother
+proving progress again so I included them in the rules *)
+Inductive step : term -> term -> Prop :=
+| EApp1 : forall t1 t1' t2, ~(value t1) ->
+                       step t1 t1' -> step (TApp t1 t2) (TApp t1' t2)
+| EApp2 : forall v1 t2 t2', value v1 ->
+                       ~(value t2) ->
+                       step t2 t2' -> step (TApp v1 t2) (TApp v1 t2')
+| EAppAbs : forall x t1 v2, value v2 ->
+                       step (TApp (TLam x t1) v2) (sub t1 x v2)
+.
+Hint Constructors step.
+
+Inductive multi_step : term -> term -> Prop :=
+| MS0 : forall t, multi_step t t
+| MSs : forall t t' t'', step t t' -> multi_step t' t'' -> multi_step t t''.
+
+Inductive evals_to : term -> term -> Prop :=
+| EtVal : forall t, value t -> evals_to t t
+| EtStep : forall t t' t'', step t t' -> evals_to t' t'' -> evals_to t t''.
+Hint Constructors evals_to.
+
+Lemma evals_to_trans : forall a b c, evals_to a b -> evals_to b c -> evals_to a c.
+Proof.
+  intros a b c H.
+  generalize dependent c.
+  induction H; intros.
+  - auto.
+  - apply IHevals_to in H1. eauto.
+Qed.
+Hint Resolve evals_to_trans.
+
+Lemma evals_to_app : forall a b a' b',
+    evals_to a a' -> evals_to b b' -> evals_to (TApp a b) (TApp a' b').
+Proof.
+  intros.
+  induction H.
+  - induction H0.
+    + auto.
+    + apply evals_to_trans.
+
+
+Definition halting (t: term) : Prop := exists v, evals_to t v.
+Hint Unfold halting.
+
+Definition x := "x".
+Example omega_ := TApp (TLam x (TApp x x)) (TLam x (TApp x x)).
+
+Example omega_non_halting : ~(halting omega_).
+Proof.
+  unfold omega_.
+  unfold halting.
+  intro.
+  remember (TApp (TLam x (TApp x x)) (TLam x (TApp x x))) as omega_.
+  destruct H as [v].
+  induction H; intros; subst.
+  - inversion H.
+  - inversion H.
+    + subst. apply H3. easy.
+    + subst. apply H4. easy.
+    + subst. apply IHevals_to. easy.
+Qed.
+
+(* church encoding for true and false *)
+Definition tru_ := TLam "a" (TLam "b" "a").
+Definition fls_ := TLam "a" (TLam "b" "b").
+Definition if_ := TLam "p" (TLam "a" (TLam "b" (TApp (TApp "p" "a") "b"))).
+
+Lemma if_tru_fls : forall cond t f,
+    (evals_to cond tru_ -> evals_to (TApp (TApp (TApp if_ cond) t) f) t) /\
+    (evals_to cond fls_ -> evals_to (TApp (TApp (TApp if_ cond) t) f) f).
+Proof.
+  intros.
+  unfold if_, tru_, fls_.
+  split.
+  - (* case: cond evals_to true *)
+    intro.
+    apply evals_to_trans with (b := (TApp (TApp tru_ t) f)).
+    eapply evals_to_trans.
+
+    (* apply evals_to_trans with (b := (TApp (TApp tru_ t) f)). *)
+
+
+    eapply EtStep.
+    eapply EApp1; auto.
+    eapply EApp1; auto.
+  - (* case: cond evals_to false *)
+
+
+Definition oracle (o: term) :=
+  forall t input, (evals_to (TApp (TApp o t) input) tru_ \/
+              evals_to (TApp (TApp o t) input) fls_)
+             /\ (evals_to (TApp (TApp o t) input) tru_ <->
+                halting (TApp t input))
+             /\ (evals_to (TApp (TApp o t) input) fls_ <->
+                ~(halting (TApp t input))).
+
+Definition problematic (oracle: term) :=
+  TLam "i" (TApp (TApp (TApp if_ (TApp oracle "i")) omega_) tru_).
+
+Lemma problematic_property :
+  forall m, halting (problematic m) -> evals_to (problematic m) tru_.
+Proof.
+  intros.
+  unfold problematic in *.
+  destruct H.
+  eapply EtStep.
+
+
+
+(* halting problem *)
+Theorem halting_problem : ~exists o, oracle o.
+Proof.
+  unfold oracle.
+  intro.
+  destruct H as [oracle].
+  remember (
+      (* λi.if_ (halts i) then omega_ else tru *)
+      TLam "i" (TApp (TApp (TApp if_ (TApp oracle "i")) omega_) tru_)
+    )
+    as problematic.
+  pose proof (H problematic problematic).
+  clear H.
+  destruct H0 as [[Hch | Hcnh] [Hh Hnh]].
+  - (* Case 1: problematic halts on problematic *)
+    apply Hh in Hch.
+    unfold halting in Hch.
+    destruct Hch.
+    inversion H
